theories/Substitution.v
@@ -38,64 +38,7 @@ Class Subst (A : OType) : Type :=
   subst : forall {Θ}, ⊧ A ↠ Box Θ A.
 #[global] Arguments subst {_ _ _} [w] _ [_] _.
 
-#[export] Instance subst_ty : Subst OTy :=
-  fun Θ =>
-    fix subst {w0} (t : OTy w0) {w1} θ : OTy w1 :=
-      match t with
-      | oty.evar αIn   => lk θ αIn
-      | oty.bool       => oty.bool
-      | oty.func t1 t2 => oty.func (subst t1 θ) (subst t2 θ)
-      end.
-
-#[export] Instance subst_env : Subst OEnv.
-Proof.
-  intros Θ w0 Γ w1 θ. revert Γ.
-  unfold OEnv. eapply base.fmap.
-  intros t. apply (subst t θ).
-Defined.
-
-Class LkRefl (Θ : SUB) (reflΘ : Refl Θ) : Prop :=
-  lk_refl w α (αIn : α ∈ w) :
-    lk refl αIn = oty.evar αIn.
-#[global] Arguments LkRefl Θ {_}.
-Class LkTrans (Θ : SUB) (transΘ : Trans Θ) : Prop :=
-  lk_trans w0 w1 w2 (θ1 : Θ w0 w1) (θ2 : Θ w1 w2) α (αIn : α ∈ w0) :
-    lk (trans θ1 θ2) αIn = subst (lk θ1 αIn) θ2.
-#[global] Arguments LkRefl Θ {_}.
-#[global] Arguments LkTrans Θ {_}.
-
-Class LkHMap (Θ1 Θ2 : SUB) (hmapΘ : HMap Θ1 Θ2) : Prop :=
-  lk_hmap [w1 w2] (θ : Θ1 w1 w2) :
-    ∀ α (αIn : α ∈ w1), lk (hmap θ) αIn = lk θ αIn.
-#[global] Arguments LkHMap Θ1 Θ2 {_}.
-
-Class SubstLaws A {subA : Subst A} : Type :=
-  { subst_refl {Θ} {reflΘ : Refl Θ} {lkreflΘ : LkRefl Θ} :
-      forall w (a : A w),
-        subst a (refl (Θ := Θ)) = a;
-    subst_trans {Θ : SUB} {transΘ : Trans Θ} {lktransΘ : LkTrans Θ} :
-      forall w0 (a : A w0) w1 (θ1 : Θ w0 w1) w2 (θ2 : Θ w1 w2),
-        subst a (trans θ1 θ2) = subst (subst a θ1) θ2;
-    subst_simulation {Θ1 Θ2 : SUB} :
-      forall w0 a w1 (θ1 : Θ1 w0 w1) (θ2 : Θ2 w0 w1),
-        (forall α (αIn : α ∈ w0), lk θ1 αIn = lk θ2 αIn) ->
-        subst a θ1 = subst a θ2;
-  }.
-#[global] Arguments SubstLaws A {_}.
-
-#[export] Instance substlaws_ty : SubstLaws OTy.
-Proof.
-  constructor.
-  - intros * ? w t. induction t; cbn.
-    + apply lk_refl.
-    + reflexivity.
-    + now f_equal.
-  - intros * ? w0 t *. induction t; cbn.
-    + apply lk_trans.
-    + reflexivity.
-    + now f_equal.
-  - intros ? ? ? t * Heq. induction t; cbn; f_equal; auto.
-Qed.
+Load SubstitutionStlcInstances.
 
 #[export] Instance subst_unit : Subst Unit :=
   fun Θ w1 u w2 r => u.
@@ -109,14 +52,31 @@ Qed.
   Subst (List A) :=
   fun Θ w1 la w2 r => List.map (fun a => subst a r) la.
 
-#[export] Instance substlaws_option {A} `{subLawsA : SubstLaws A} :
-  SubstLaws (Option A).
-Proof.
-  constructor.
-  - intros. destruct a; cbn; f_equal. apply subst_refl.
-  - intros. destruct a; cbn; f_equal. apply subst_trans.
-  - intros. destruct a; cbn; f_equal. now apply subst_simulation.
-Qed.
+Class LkRefl (Θ : SUB) (reflΘ : Refl Θ) : Prop :=
+  lk_refl w α (αIn : α ∈ w) :
+    lk refl αIn = oty.evar αIn.
+#[global] Arguments LkRefl Θ {_}.
+Class LkTrans (Θ : SUB) (transΘ : Trans Θ) : Prop :=
+  lk_trans w0 w1 w2 (θ1 : Θ w0 w1) (θ2 : Θ w1 w2) α (αIn : α ∈ w0) :
+    lk (trans θ1 θ2) αIn = subst (lk θ1 αIn) θ2.
+#[global] Arguments LkRefl Θ {_}.
+#[global] Arguments LkTrans Θ {_}.
+
+Class SubstLaws A {subA : Subst A} : Type :=
+  { subst_refl {Θ} {reflΘ : Refl Θ} {lkreflΘ : LkRefl Θ} :
+    forall w (a : A w),
+      subst a (refl (Θ := Θ)) = a;
+    subst_trans {Θ : SUB} {transΘ : Trans Θ} {lktransΘ : LkTrans Θ} :
+    forall w0 (a : A w0) w1 (θ1 : Θ w0 w1) w2 (θ2 : Θ w1 w2),
+      subst a (trans θ1 θ2) = subst (subst a θ1) θ2;
+    subst_simulation {Θ1 Θ2 : SUB} :
+    forall w0 a w1 (θ1 : Θ1 w0 w1) (θ2 : Θ2 w0 w1),
+      (forall α (αIn : α ∈ w0), lk θ1 αIn = lk θ2 αIn) ->
+      subst a θ1 = subst a θ2;
+  }.
+#[global] Arguments SubstLaws A {_}.
+
+Load SubstitutionStlcProofs.
 
 #[export] Instance substlaws_prod {A B} `{SubstLaws A, SubstLaws B} :
   SubstLaws (Prod A B).
@@ -126,56 +86,16 @@ Proof.
   - intros. destruct a; cbn; f_equal; apply subst_trans.
   - intros. destruct a; cbn; f_equal; now apply subst_simulation.
 Qed.
-
-#[export] Instance substlaws_env : SubstLaws OEnv.
+#[export] Instance substlaws_option {A} `{subLawsA : SubstLaws A} :
+  SubstLaws (Option A).
 Proof.
   constructor.
-  - intros * ? w Γ. unfold subst, subst_env, OEnv.
-    apply map_eq. intros x. rewrite lookup_fmap.
-    destruct lookup as [t|]; cbn; f_equal.
-    apply subst_refl.
-  - intros * ? w0 Γ *. unfold subst, subst_env, OEnv.
-    apply map_eq. intros x. rewrite !lookup_fmap.
-    destruct lookup as [t|]; cbn; f_equal.
-    apply subst_trans.
-  - intros ? ? ? t * Heq. unfold subst, subst_env.
-    apply (map_fmap_ext _ _ t). intros x s _. clear - Heq.
-    now apply subst_simulation.
+  - intros. destruct a; cbn; f_equal. apply subst_refl.
+  - intros. destruct a; cbn; f_equal. apply subst_trans.
+  - intros. destruct a; cbn; f_equal. now apply subst_simulation.
 Qed.
-
-(* #[export] Instance Subst_In {x} : *)
-(*   Subst Alloc (ctx.In x) := *)
-(*   fix transient {w} (xIn : x ∈ w) {w'} (r : Alloc w w') {struct r} := *)
-(*     match r with *)
-(*     | alloc.refl _        => xIn *)
-(*     | alloc.fresh _ α _ r => transient (in_succ xIn) r *)
-(*     end. *)
-
-(* #[export] Instance SubstLaws_In {x} : SubstLaws (ctx.In x). *)
-(* Proof. constructor; [easy|induction r12; cbn; auto]. Qed. *)
-
 #[export] Instance subst_const {A} : Subst (Const A) :=
   fun _ _ a _ _ => a.
-
-Lemma lookup_subst {Θ : SUB}
-  {w0 w1} (θ : Θ w0 w1) (G : OEnv w0) (x : string) :
-  lookup x (subst G θ) = subst (lookup x G) θ.
-Proof.
-  unfold subst at 1, subst_env, OEnv.
-  now rewrite lookup_fmap.
-Qed.
-
-Lemma subst_empty {Θ : SUB}
-  {w0 w1} (θ : Θ w0 w1) :
-  subst (empty (A := OEnv w0)) θ = empty.
-Proof.
-  apply (fmap_empty (M := gmap string)).
-Qed.
-
-Lemma subst_insert {Θ : SUB}
-  {w0 w1} (θ : Θ w0 w1) (G : OEnv w0) (x : string) (t : OTy w0) :
-  subst (insert x t G) θ = insert x (subst t θ) (subst G θ).
-Proof. unfold subst, subst_env, OEnv. now rewrite fmap_insert. Qed.
 
 Class LkStep (Θ : SUB) (stepΘ : Step Θ) : Prop :=
   lk_step w α (αIn : α ∈ w) β :
@@ -191,3 +111,8 @@ Class LkThick (Θ : SUB) (thickΘ : Thick Θ) : Prop :=
   lk_thick w α (αIn : α ∈ w) (t : OTy (w - α)) β (βIn : β ∈ w) :
     lk (thick α t) βIn = thickIn αIn t βIn.
 #[global] Arguments LkThick Θ {_}.
+
+Class LkHMap (Θ1 Θ2 : SUB) (hmapΘ : HMap Θ1 Θ2) : Prop :=
+  lk_hmap [w1 w2] (θ : Θ1 w1 w2) :
+    ∀ α (αIn : α ∈ w1), lk (hmap θ) αIn = lk θ αIn.
+#[global] Arguments LkHMap Θ1 Θ2 {_}.
