theories/SubstitutionStlcProofs.v
@@ -26,20 +26,52 @@
 (* SOFTWARE, EVEN IF ADVISED OF THE POSSIBILITY OF SUCH DAMAGE.               *)
 (******************************************************************************)
 
-From Coq Require Import ExtrHaskellBasic ExtrHaskellNatInt ExtrHaskellString Bool.
-From Em Require Import Composition.
+#[export] Instance substlaws_ty : SubstLaws OTy.
+Proof.
+  constructor.
+  - intros * ? w t. induction t; cbn.
+    + apply lk_refl.
+    + reflexivity.
+    + now f_equal.
+  - intros * ? w0 t *. induction t; cbn.
+    + apply lk_trans.
+    + reflexivity.
+    + now f_equal.
+  - intros ? ? ? t * Heq. induction t; cbn; f_equal; auto.
+Qed.
 
-Extraction Language Haskell.
-Extraction Inline Bool.Bool.iff_reflect Environment.env.view
-  Init.Datatypes.nat_rec Init.Logic.False_rec Init.Logic.and_rec
-  Init.Logic.and_rect Init.Logic.eq_rec_r Init.Specif.sumbool_rec
-  Init.Specif.sumbool_rect Unification.atrav Unification.flex
-  Unification.loeb Unification.remove_acc_rect Unification.varview
-  Worlds.Box Worlds.Impl Worlds.Impl Worlds.Valid Worlds.lk Worlds._4
-  Worlds.world.view stdpp.base.empty stdpp.base.insert stdpp.base.fmap
-  stdpp.base.decide_rel stdpp.gmap.gmap_fmap stdpp.option.option_fmap.
+#[export] Instance substlaws_env : SubstLaws OEnv.
+Proof.
+  constructor.
+  - intros * ? w Γ. unfold subst, subst_env, OEnv.
+    apply map_eq. intros x. rewrite lookup_fmap.
+    destruct lookup as [t|]; cbn; f_equal.
+    apply subst_refl.
+  - intros * ? w0 Γ *. unfold subst, subst_env, OEnv.
+    apply map_eq. intros x. rewrite !lookup_fmap.
+    destruct lookup as [t|]; cbn; f_equal.
+    apply subst_trans.
+  - intros ? ? ? t * Heq. unfold subst, subst_env.
+    apply (map_fmap_ext _ _ t). intros x s _. clear - Heq.
+    now apply subst_simulation.
+Qed.
 
-Extract Inductive reflect => "Prelude.Bool" [ "Prelude.True" "Prelude.False" ].
-Extract Inlined Constant Init.Datatypes.fst => "Prelude.fst".
-Extract Inlined Constant Init.Datatypes.snd => "Prelude.snd".
-Extraction "Extract" ground_type ground_expr infer_free infer_prenex infer_solved.
+Lemma lookup_subst {Θ : SUB}
+  {w0 w1} (θ : Θ w0 w1) (G : OEnv w0) (x : string) :
+  lookup x (subst G θ) = subst (lookup x G) θ.
+Proof.
+  unfold subst at 1, subst_env, OEnv.
+  now rewrite lookup_fmap.
+Qed.
+
+Lemma subst_empty {Θ : SUB}
+  {w0 w1} (θ : Θ w0 w1) :
+  subst (empty (A := OEnv w0)) θ = empty.
+Proof.
+  apply (fmap_empty (M := gmap string)).
+Qed.
+
+Lemma subst_insert {Θ : SUB}
+  {w0 w1} (θ : Θ w0 w1) (G : OEnv w0) (x : string) (t : OTy w0) :
+  subst (insert x t G) θ = insert x (subst t θ) (subst G θ).
+Proof. unfold subst, subst_env, OEnv. now rewrite fmap_insert. Qed.
